theories/Fundamental.v
@@ -230,10 +230,7 @@ Section Fundamental.
   Proof.
   Admitted.
 
-  (* FIXME *)
-  Notation "x × y" := (Datatypes.prod x y) (at level 80, right associativity).
-
-  Lemma Fundamental : (forall Γ : context, [ |-[ de ] Γ ] -> FundCon (ta := ta) Γ)
+Lemma Fundamental : (forall Γ : context, [ |-[ de ] Γ ] -> FundCon (ta := ta) Γ)
     × (forall (Γ : context) (A : term), [Γ |-[ de ] A] -> FundTy (ta := ta) Γ A)
     × (forall (Γ : context) (A t : term), [Γ |-[ de ] t : A] -> FundTm (ta := ta) Γ A t)
     × (forall (Γ : context) (A B : term), [Γ |-[ de ] A ≅ B] -> FundTyEq (ta := ta) Γ A B)
